calc/semantics.v
@@ -45,31 +45,31 @@ Lemma LiftLambdaTest : (LiftLambda TNat (App (VAR 1 : TNat ==> TNat) (VAR 0 : TN
 Qed.
 
 
-(* I don't check if the term is plain, I just assume it in the reduction rule before using Match *)
-Definition Match (t : typedterm) (p : pattrn) : option (typedterm -> typedterm) :=
-  match (t, p) with
-  | (Nat n : TNat, PNatLit n') =>
-    if Nat.eq_dec n n' then
-      Some (fun t => t)
-    else None
-  | (VAR x : T,  PVar x') =>
-    if Nat.eq_dec x x' then
-      Some (fun t => t)
-    else None
-(* TODO  fixpoint *)
-  | (App (e1 : T1) (e2 : T2) : T,  PBindApp T1' T2') =>
-    if (type_beq T1 T1') && (type_beq T2 T2') then
-      Some (fun t => t.[Quote (e2 : T2) : □T2/].[Quote (e1 : T1) : □T1/])
-    else None
-  | (Nat n : TNat, PBindUnlift) =>
-    Some (fun t => t.[Nat n : TNat/])
-  | (Lam argT body : T1 ==> T2, PBindLam T) =>
-    if type_beq (T1 ==> T2) T && type_beq argT T1 then
-      let lifted := LiftLambda argT body T2 in
-      Some (fun t => t.[lifted/])
-    else None
-  | _ => None
-  end.
+(* (* I don't check if the term is plain, I just assume it in the reduction rule before using Match *) *)
+(* Definition Match (t : typedterm) (p : pattrn) : option (typedterm -> typedterm) := *)
+(*   match (t, p) with *)
+(*   | (Nat n : TNat, PNatLit n') => *)
+(*     if Nat.eq_dec n n' then *)
+(*       Some (fun t => t) *)
+(*     else None *)
+(*   | (VAR x : T,  PVar x') => *)
+(*     if Nat.eq_dec x x' then *)
+(*       Some (fun t => t) *)
+(*     else None *)
+(* (* TODO  fixpoint *) *)
+(*   | (App (e1 : T1) (e2 : T2) : T,  PBindApp T1' T2') => *)
+(*     if (type_beq T1 T1') && (type_beq T2 T2') then *)
+(*       Some (fun t => t.[Quote (e2 : T2) : □T2/].[Quote (e1 : T1) : □T1/]) *)
+(*     else None *)
+(*   | (Nat n : TNat, PBindUnlift) => *)
+(*     Some (fun t => t.[Nat n : TNat/]) *)
+(*   | (Lam argT body : T1 ==> T2, PBindLam T) => *)
+(*     if type_beq (T1 ==> T2) T && type_beq argT T1 then *)
+(*       let lifted := LiftLambda argT body T2 in *)
+(*       Some (fun t => t.[lifted/]) *)
+(*     else None *)
+(*   | _ => None *)
+(*   end. *)
 
 Reserved Notation "t1 '-->(' L ')' t2" (at level 48).
 Inductive reducts : Level -> typedterm -> typedterm -> Prop :=
@@ -81,15 +81,74 @@ Inductive reducts : Level -> typedterm -> typedterm -> Prop :=
     isplain t -> (Splice (Quote t : □T) : T) -->(L1) t
 | E_Lift_Red : forall n TN T,
     (Lift (Nat n : TN) : T) -->(L0) (Quote (Nat n : TN) : T)
-| E_Pat_Succ : forall t Ts T p s f σ s',
+| E_PatNat_Succ : forall n t t' T s f,
+    t = (Nat n : TNat) ->
     isplain t ->
-    Match t p = Some σ ->
-    s' = σ(s) ->
-    (PatternMatch (Quote t : □Ts) p s f : T) -->(L0) s'
-| E_Pat_Fail : forall t Ts T p s f,
+    t' = (Quote t : □TNat) ->
+    (MatchNat t' n s f : T) -->(L0) s
+| E_PatNat_Red : forall t t' n T s f,
+    t -->(L0) t' ->
+    (MatchNat t n s f : T) -->(L0) (MatchNat t' n s f : T)
+| E_PatNat_Fail : forall n t t' T s f,
     isplain t ->
-    Match t p = None ->
-    (PatternMatch (Quote t : □Ts) p s f : T) -->(L0) f
+    t <> (Nat n : TNat) ->
+    t' = (Quote t : □TNat) ->
+    (MatchNat t' n s f : T) -->(L0) f
+| E_PatVar_Succ : forall x t t' T1 T s f,
+    t = (VAR x : T1) ->
+    isplain t ->
+    t' = (Quote t : □T1) ->
+    (MatchVar t' (VAR x) s f : T) -->(L0) s
+| E_PatVar_Red : forall t t' x T s f,
+    t -->(L0) t' ->
+    (MatchVar t (VAR x) s f : T) -->(L0) (MatchVar t' (VAR x) s f : T)
+| E_PatVar_Fail : forall x t t' T1 T s f,
+    isplain t ->
+    t <> (VAR x : T1) ->
+    t' = (Quote t : □T1) ->
+    (MatchVar t' (VAR x) s f : T) -->(L0) f
+| E_PatApp_Succ : forall t t' e1 T1 e2 T2 T3 T s s' f,
+    t = (App (e1 : T1) (e2 : T2) : T3) ->
+    isplain t ->
+    t' = (Quote t : □T3) ->
+    s' = s.[Quote (e2 : T2) : □T2/].[Quote (e1 : T1) : □T1/] ->
+    (MatchApp t' T1 T2 s f : T) -->(L0) s'
+| E_PatApp_Red : forall t t' T1 T2 T s f,
+    t -->(L0) t' ->
+    (MatchApp t T1 T2 s f : T) -->(L0) (MatchApp t' T1 T2 s f : T)
+| E_PatApp_Fail : forall t t' e1 T1 e2 T2 T3 T s f,
+    t <> (App (e1 : T1) (e2 : T2) : T3) ->
+    isplain t ->
+    t' = (Quote t : □T3) ->
+    (MatchApp t' T1 T2 s f : T) -->(L0) f
+| E_PatUnlift_Succ : forall t t' n T s s' f,
+    t = (Nat n : TNat) ->
+    isplain t ->
+    t' = (Quote t : □TNat) ->
+    s' = s.[Nat n : TNat/] ->
+    (MatchUnlift t' s f : T) -->(L0) s'
+| E_PatUnlift_Red : forall t t' T s f,
+    t -->(L0) t' ->
+    (MatchUnlift t s f : T) -->(L0) (MatchUnlift t' s f : T)
+| E_PatUnlift_Fail : forall t t' n T s f,
+    isplain t ->
+    t <> (Nat n : TNat) ->
+    t' = (Quote t : □TNat) ->
+    (MatchUnlift t' s f : T) -->(L0) f
+| E_PatLam_Succ : forall t t' T1 body T2 T s s' f,
+    t = (Lam T1 body : T1 ==> T2) ->
+    isplain t ->
+    t' = (Quote t : □(T1 ==> T2)) ->
+    s' = s.[LiftLambda T1 body T2/] ->
+    (MatchApp t' T1 T2 s f : T) -->(L0) s'
+| E_PatLam_Red : forall t t' T1 T s f,
+    t -->(L0) t' ->
+    (MatchLam t T1 s f : T) -->(L0) (MatchLam t' T1 s f : T)
+| E_PatLam_Fail : forall t t' T1 body T2 T s f,
+    t <> (Lam T1 body : T1 ==> T2) ->
+    isplain t ->
+    t' = (Quote t : □(T1 ==> T2)) ->
+    (MatchApp t' T1 T2 s f : T) -->(L0) f
 | E_App1 : forall L t1 t2 t1' T, t1 -->(L) t1' -> (App t1 t2 : T) -->(L) (App t1' t2 : T)
 | E_App2 : forall L t1 t2 t2' T, t2 -->(L) t2' -> (App t1 t2 : T) -->(L) (App t1 t2' : T)
 | E_Abs : forall t t' T1 T,
@@ -106,9 +165,6 @@ Inductive reducts : Level -> typedterm -> typedterm -> Prop :=
     (Lift t : T) -->(L0) (Lift t' : T)
 (* | E_Fix : TODO *)
 (* | E_Fix_Red : TODO *)
-| E_Pat : forall T t1 p s f t1',
-    t1 -->(L0) t1' ->
-    (PatternMatch t1 p s f : T) -->(L0) (PatternMatch t1' p s f : T)
 where "t1 '-->(' L ')' t2" := (reducts L t1 t2).
 Hint Constructors reducts.
 
